specs/Spec.Lib.IntVec.fst
@@ -1,0 +1,56 @@
+module Spec.Lib.IntVec
+
+open Spec.Lib.IntTypes
+open FStar.Seq
+open FStar.Mul
+let bits vt = bits vt.t
+let size vt = size vt.t * vt.len
+
+type intvec (vt:vectype) = 
+  s:seq (uint_t vt.t){length s = vt.len}
+  
+let vec_add #vt (v1:intvec vt) (v2:intvec vt) : intvec vt = 
+Spec.Loops.seq_map2 (add_mod #vt.t) v1 v2
+
+let vec_sub #vt (v1:intvec vt) (v2:intvec vt) : intvec vt = 
+Spec.Loops.seq_map2 (sub_mod #vt.t) v1 v2
+
+let vec_mul (#vt:vectype{vt.t <> U128}) (v1:intvec vt) (v2:intvec vt): intvec vt = 
+Spec.Loops.seq_map2 (mul_mod #vt.t) v1 v2
+
+let vec_xor #vt (v1:intvec vt) (v2:intvec vt) : intvec vt = 
+Spec.Loops.seq_map2 (logxor #vt.t) v1 v2
+
+let vec_and #vt (v1:intvec vt) (v2:intvec vt) : intvec vt = 
+Spec.Loops.seq_map2 (logand #vt.t) v1 v2
+
+let vec_or #vt (v1:intvec vt) (v2:intvec vt) : intvec vt = 
+Spec.Loops.seq_map2 (logor #vt.t) v1 v2
+
+let vec_not #vt (v1:intvec vt) : intvec vt = 
+Spec.Loops.seq_map (lognot #vt.t) v1 
+
+let vec_shift_right #vt v1 s = 
+Spec.Loops.seq_map (fun x -> shift_right x s) v1 
+
+let vec_shift_left #vt (v1:intvec vt) (s:uint32{uint_v s < bits vt}) : intvec vt = 
+Spec.Loops.seq_map (fun x -> shift_left #vt.t x s) v1 
+
+let vec_rotate_right #vt (v1:intvec vt) (s:uint32{uint_v s > 0 /\ uint_v s < bits vt}) : intvec vt = 
+Spec.Loops.seq_map (fun x -> rotate_right  #vt.t x s) v1 
+
+let vec_rotate_left #vt (v1:intvec vt) (s:uint32{uint_v s > 0 /\ uint_v s < bits vt}) : intvec vt = 
+Spec.Loops.seq_map (fun x -> rotate_left #vt.t x s) v1 
+
+let op_Plus_Bar = vec_add
+let op_Subtraction_Bar = vec_sub
+let op_Star_Bar = vec_mul
+let op_Hat_Bar = vec_xor
+let op_Amp_Bar = vec_and
+let op_Bar_Bar = vec_or
+let op_Tilde_Bar = vec_not
+let op_Greater_Greater_Bar = vec_shift_right
+let op_Less_Less_Bar = vec_shift_left
+let op_Greater_Greater_Greater_Bar = vec_rotate_right
+let op_Less_Less_Less_Bar = vec_rotate_left
+
