specs/Spec.Lib.IntVec.fsti
@@ -1,0 +1,42 @@
+module Spec.Lib.IntVec
+
+open Spec.Lib.IntTypes
+open FStar.Seq
+open FStar.Mul
+
+type vectype = 
+  | V: t:inttype -> len:nat -> vectype
+val bits: vt:vectype -> n:nat{n = bits vt.t}
+val size: vt:vectype -> n:nat{n = size vt.t * vt.len}
+
+val intvec: vt:vectype -> Type0
+
+val vec_add: #vt:vectype -> intvec vt -> intvec vt -> intvec vt
+val vec_sub: #vt:vectype -> intvec vt -> intvec vt -> intvec vt
+val vec_mul: #vt:vectype{vt.t <> U128} -> intvec vt -> intvec vt -> intvec vt
+val vec_xor: #vt:vectype -> intvec vt -> intvec vt -> intvec vt
+val vec_and: #vt:vectype -> intvec vt -> intvec vt -> intvec vt
+val vec_or: #vt:vectype -> intvec vt -> intvec vt -> intvec vt
+val vec_not: #vt:vectype -> intvec vt -> intvec vt
+
+val vec_shift_right: #vt:vectype -> intvec vt -> (s:uint32{uint_v s < bits vt}) -> intvec vt
+val vec_shift_left: #vt:vectype -> intvec vt -> (s:uint32{uint_v s < bits vt}) -> intvec vt
+val vec_rotate_right: #vt:vectype -> intvec vt -> (s:uint32{uint_v s > 0 /\ uint_v s < bits vt}) -> intvec vt
+val vec_rotate_left: #vt:vectype -> intvec vt -> (s:uint32{uint_v s > 0 /\ uint_v s < bits vt}) -> intvec vt
+
+
+
+val ( +| ): #vt:vectype -> intvec vt -> intvec vt -> intvec vt
+val ( -| ): #vt:vectype -> intvec vt -> intvec vt -> intvec vt
+val ( *| ): #vt:vectype{vt.t <> U128} -> intvec vt -> intvec vt -> intvec vt
+val ( ^| ): #vt:vectype -> intvec vt -> intvec vt -> intvec vt
+val ( &| ): #vt:vectype -> intvec vt -> intvec vt -> intvec vt
+val ( || ): #vt:vectype -> intvec vt -> intvec vt -> intvec vt
+val ( ~| ): #vt:vectype -> intvec vt -> intvec vt
+
+val ( >>| ): #vt:vectype -> intvec vt -> (s:uint32{uint_v s < bits vt}) -> intvec vt
+val ( <<| ): #vt:vectype -> intvec vt -> (s:uint32{uint_v s < bits vt}) -> intvec vt
+val ( >>>| ): #vt:vectype -> intvec vt -> (s:uint32{uint_v s > 0 /\ uint_v s < bits vt}) -> intvec vt
+val ( <<<| ): #vt:vectype -> intvec vt -> (s:uint32{uint_v s > 0 /\ uint_v s < bits vt}) -> intvec vt
+
+
